# baseURI: https://www.tno.nl/agrifood/ontology/greenhouse-model/
# imports: https://raw.githubusercontent.com/HajoRijgersberg/OM/master/om-2.0.rdf
# prefix: ghm

@prefix MathM: <http://www.w3.org/1998/Math/MathML> .
@prefix ghm: <https://www.tno.nl/agrifood/ontology/greenhouse-model/> .
@prefix owl: <http://www.w3.org/2002/07/owl#> .
@prefix rdf: <http://www.w3.org/1999/02/22-rdf-syntax-ns#> .
@prefix rdfs: <http://www.w3.org/2000/01/rdf-schema#> .
@prefix spin: <http://spinrdf.org/spin#> .
@prefix um: <http://www.ontology-of-units-of-measure.org/resource/om-2/> .
@prefix xml: <http://www.w3.org/XML/1998/namespace> .
@prefix xsd: <http://www.w3.org/2001/XMLSchema#> .

owl:Thing
  rdf:type owl:Class ;
.
ghm:
  rdf:type owl:Ontology ;
  spin:imports <http://topbraid.org/spin/owlrl-all> ;
  owl:imports <https://raw.githubusercontent.com/HajoRijgersberg/OM/master/om-2.0.rdf> ;
.
ghm:Block
  rdf:type owl:Class ;
  rdfs:comment "A block contains only a single crop (this is a requirement)" ;
  rdfs:comment "A block is part of a compartment in the greenhouse in which the plants are treated equally wrt nutrition, climate etc." ;
  rdfs:comment "Each block has a unique identifier in the greenhouse or compartment in the greenhouse" ;
  rdfs:comment "This class represents blocks that are part of a greenhouse and contain a set of plants" ;
  rdfs:label "Block" ;
  rdfs:subClassOf owl:Thing ;
  rdfs:subClassOf [
      rdf:type owl:Restriction ;
      owl:cardinality "1"^^xsd:nonNegativeInteger ;
      owl:onProperty ghm:hasBlockIdentifier ;
    ] ;
  rdfs:subClassOf [
      rdf:type owl:Restriction ;
      owl:onClass ghm:Crop ;
      owl:onProperty ghm:contains ;
      owl:qualifiedCardinality "1"^^xsd:nonNegativeInteger ;
    ] ;
.
ghm:Builder
  rdf:type owl:Class ;
  rdfs:comment "This class represents builders that build greenhouses and possibly support growers in their crop management activities" ;
  rdfs:label "Builder" ;
  rdfs:subClassOf owl:Thing ;
.
ghm:Compartment
  rdf:type owl:Class ;
  rdfs:comment "A compartment is a part of the greenhouse" ;
  rdfs:comment "Each compartment has a unique identifier in the greenhouse" ;
  rdfs:comment "This class represents compartments that are part of a greenhouse and contain a set of plants" ;
  rdfs:label "Block" ;
  rdfs:subClassOf owl:Thing ;
  rdfs:subClassOf [
      rdf:type owl:Restriction ;
      owl:onProperty ghm:contains ;
      owl:someValuesFrom ghm:Block ;
    ] ;
  rdfs:subClassOf [
      rdf:type owl:Restriction ;
      owl:onProperty ghm:contains ;
      owl:someValuesFrom ghm:Zone ;
    ] ;
.
ghm:Crop
  rdf:type owl:Class ;
  rdfs:comment "More characteristics of a crop can be defined using the guideline for creating a crop ontology published here: http://www.cropontology.org" ;
  rdfs:comment "This class represents crops that are produced in a greenhouse operated by a grower" ;
  rdfs:label "Crop" ;
  rdfs:subClassOf owl:Thing ;
  rdfs:subClassOf [
      rdf:type owl:Restriction ;
      owl:cardinality "1"^^xsd:nonNegativeInteger ;
      owl:onProperty ghm:hasName ;
    ] ;
  rdfs:subClassOf [
      rdf:type owl:Restriction ;
      owl:onProperty ghm:isGrownBy ;
      owl:someValuesFrom ghm:Grower ;
    ] ;
  rdfs:subClassOf [
      rdf:type owl:Restriction ;
      owl:onProperty ghm:isGrownIn ;
      owl:someValuesFrom ghm:Greenhouse ;
    ] ;
.
ghm:DisinfectionSystem
  rdf:type owl:Class ;
  rdfs:label "Disinfection system" ;
  rdfs:subClassOf ghm:WaterSystem ;
.
ghm:Greenhouse
  rdf:type owl:Class ;
  rdfs:comment "This class represents greenhouses in which crop is being grown by a grower" ;
  rdfs:label "Greenhouse" ;
  rdfs:subClassOf owl:Thing ;
  rdfs:subClassOf [
      rdf:type owl:Restriction ;
      owl:onClass ghm:Builder ;
      owl:onProperty ghm:isBuildBy ;
      owl:qualifiedCardinality "1"^^xsd:nonNegativeInteger ;
    ] ;
  rdfs:subClassOf [
      rdf:type owl:Restriction ;
      owl:onClass ghm:Grower ;
      owl:onProperty ghm:isOperatedBy ;
      owl:qualifiedCardinality "1"^^xsd:nonNegativeInteger ;
    ] ;
  rdfs:subClassOf [
      rdf:type owl:Restriction ;
      owl:onProperty ghm:contains ;
      owl:someValuesFrom ghm:Compartment ;
    ] ;
  rdfs:subClassOf [
      rdf:type owl:Restriction ;
      owl:onProperty ghm:contains ;
      owl:someValuesFrom ghm:System ;
    ] ;
  rdfs:subClassOf [
      rdf:type owl:Restriction ;
      owl:onProperty ghm:containsBlocks ;
      owl:someValuesFrom ghm:Block ;
    ] ;
.
ghm:Grower
  rdf:type owl:Class ;
  rdfs:comment "This class represents growers that operate and possibly own a greenhouse to produce one or more crops as efficient and effective as possible" ;
  rdfs:label "Grower" ;
  rdfs:subClassOf owl:Thing ;
  rdfs:subClassOf [
      rdf:type owl:Restriction ;
      owl:onProperty ghm:grows ;
      owl:someValuesFrom ghm:Crop ;
    ] ;
.
ghm:IrrigationValve
  rdf:type owl:Class ;
  rdfs:comment "An irrigation valve is a switch that steers the amount of water in a zone" ;
  rdfs:label "Irrigation valve" ;
  rdfs:subClassOf ghm:Valve ;
.
ghm:IrrigtationSystem
  rdf:type owl:Class ;
  rdfs:label "Irrigtation system" ;
  rdfs:subClassOf ghm:WaterSystem ;
.
ghm:LeafJuiceAnalysis
  rdf:type owl:Class ;
  rdfs:comment "This class represents analysis on nutritions in a sample of leaf juice of plants in a greenhouse" ;
  rdfs:label "Leaf juice analysis" ;
  rdfs:subClassOf owl:Thing ;
  rdfs:subClassOf [
      rdf:type owl:Restriction ;
      owl:cardinality "1"^^xsd:nonNegativeInteger ;
      owl:onProperty ghm:hasDate ;
    ] ;
  rdfs:subClassOf [
      rdf:type owl:Restriction ;
      owl:cardinality "1"^^xsd:nonNegativeInteger ;
      owl:onProperty ghm:hasNutritionRecipe ;
    ] ;
  rdfs:subClassOf [
      rdf:type owl:Restriction ;
      owl:cardinality "1"^^xsd:nonNegativeInteger ;
      owl:onProperty ghm:hasSampleName ;
    ] ;
  rdfs:subClassOf [
      rdf:type owl:Restriction ;
      owl:cardinality "1"^^xsd:nonNegativeInteger ;
      owl:onProperty ghm:hasWeekNumber ;
    ] ;
  rdfs:subClassOf [
      rdf:type owl:Restriction ;
      owl:cardinality "1"^^xsd:nonNegativeInteger ;
      owl:onProperty ghm:ofCropPart ;
    ] ;
  rdfs:subClassOf [
      rdf:type owl:Restriction ;
      owl:onClass ghm:NutritionLevel ;
      owl:onProperty ghm:hasNutritionLevel ;
      owl:qualifiedCardinality "1"^^xsd:nonNegativeInteger ;
    ] ;
  rdfs:subClassOf [
      rdf:type owl:Restriction ;
      owl:onProperty ghm:ofCrop ;
      owl:someValuesFrom ghm:Crop ;
    ] ;
.
ghm:NutritionLevel
  rdf:type owl:Class ;
  rdfs:comment "This represents the class of nutrition levels in a sample of a fluid, e.g. water or leaf juice" ;
  rdfs:label "Nutrition level" ;
  rdfs:subClassOf owl:Thing ;
  rdfs:subClassOf [
      rdf:type owl:Restriction ;
      owl:cardinality "1"^^xsd:nonNegativeInteger ;
      owl:onProperty ghm:hasAl_level ;
    ] ;
  rdfs:subClassOf [
      rdf:type owl:Restriction ;
      owl:cardinality "1"^^xsd:nonNegativeInteger ;
      owl:onProperty ghm:hasB_level ;
    ] ;
  rdfs:subClassOf [
      rdf:type owl:Restriction ;
      owl:cardinality "1"^^xsd:nonNegativeInteger ;
      owl:onProperty ghm:hasCa_level ;
    ] ;
  rdfs:subClassOf [
      rdf:type owl:Restriction ;
      owl:cardinality "1"^^xsd:nonNegativeInteger ;
      owl:onProperty ghm:hasCl_level ;
    ] ;
  rdfs:subClassOf [
      rdf:type owl:Restriction ;
      owl:cardinality "1"^^xsd:nonNegativeInteger ;
      owl:onProperty ghm:hasCu_level ;
    ] ;
  rdfs:subClassOf [
      rdf:type owl:Restriction ;
      owl:cardinality "1"^^xsd:nonNegativeInteger ;
      owl:onProperty ghm:hasEC ;
    ] ;
  rdfs:subClassOf [
      rdf:type owl:Restriction ;
      owl:cardinality "1"^^xsd:nonNegativeInteger ;
      owl:onProperty ghm:hasFe_level ;
    ] ;
  rdfs:subClassOf [
      rdf:type owl:Restriction ;
      owl:cardinality "1"^^xsd:nonNegativeInteger ;
      owl:onProperty ghm:hasHCO3_level ;
    ] ;
  rdfs:subClassOf [
      rdf:type owl:Restriction ;
      owl:cardinality "1"^^xsd:nonNegativeInteger ;
      owl:onProperty ghm:hasK_Ca_ratio ;
    ] ;
  rdfs:subClassOf [
      rdf:type owl:Restriction ;
      owl:cardinality "1"^^xsd:nonNegativeInteger ;
      owl:onProperty ghm:hasK_level ;
    ] ;
  rdfs:subClassOf [
      rdf:type owl:Restriction ;
      owl:cardinality "1"^^xsd:nonNegativeInteger ;
      owl:onProperty ghm:hasMg_level ;
    ] ;
  rdfs:subClassOf [
      rdf:type owl:Restriction ;
      owl:cardinality "1"^^xsd:nonNegativeInteger ;
      owl:onProperty ghm:hasMn_level ;
    ] ;
  rdfs:subClassOf [
      rdf:type owl:Restriction ;
      owl:cardinality "1"^^xsd:nonNegativeInteger ;
      owl:onProperty ghm:hasMo_level ;
    ] ;
  rdfs:subClassOf [
      rdf:type owl:Restriction ;
      owl:cardinality "1"^^xsd:nonNegativeInteger ;
      owl:onProperty ghm:hasNH4_level ;
    ] ;
  rdfs:subClassOf [
      rdf:type owl:Restriction ;
      owl:cardinality "1"^^xsd:nonNegativeInteger ;
      owl:onProperty ghm:hasNO3_level ;
    ] ;
  rdfs:subClassOf [
      rdf:type owl:Restriction ;
      owl:cardinality "1"^^xsd:nonNegativeInteger ;
      owl:onProperty ghm:hasNa_level ;
    ] ;
  rdfs:subClassOf [
      rdf:type owl:Restriction ;
      owl:cardinality "1"^^xsd:nonNegativeInteger ;
      owl:onProperty ghm:hasP_level ;
    ] ;
  rdfs:subClassOf [
      rdf:type owl:Restriction ;
      owl:cardinality "1"^^xsd:nonNegativeInteger ;
      owl:onProperty ghm:hasS_level ;
    ] ;
  rdfs:subClassOf [
      rdf:type owl:Restriction ;
      owl:cardinality "1"^^xsd:nonNegativeInteger ;
      owl:onProperty ghm:hasSi_level ;
    ] ;
  rdfs:subClassOf [
      rdf:type owl:Restriction ;
      owl:cardinality "1"^^xsd:nonNegativeInteger ;
      owl:onProperty ghm:hasZn_level ;
    ] ;
  rdfs:subClassOf [
      rdf:type owl:Restriction ;
      owl:cardinality "1"^^xsd:nonNegativeInteger ;
      owl:onProperty ghm:haspH ;
    ] ;
  rdfs:subClassOf [
      rdf:type owl:Restriction ;
      owl:maxCardinality "1"^^xsd:nonNegativeInteger ;
      owl:onProperty ghm:hasN_level ;
    ] ;
  rdfs:subClassOf [
      rdf:type owl:Restriction ;
      owl:maxCardinality "1"^^xsd:nonNegativeInteger ;
      owl:onProperty ghm:hasN_total_level ;
    ] ;
  rdfs:subClassOf [
      rdf:type owl:Restriction ;
      owl:maxCardinality "1"^^xsd:nonNegativeInteger ;
      owl:onProperty ghm:hasSugar_concentration ;
    ] ;
.
ghm:PlantGrowth
  rdf:type owl:Class ;
  rdfs:comment "This class represents growth measurements of a single plant" ;
  rdfs:label "plant growth" ;
  rdfs:subClassOf [
      rdf:type owl:Restriction ;
      owl:cardinality "1"^^xsd:nonNegativeInteger ;
      owl:onProperty ghm:hasLength ;
    ] ;
  rdfs:subClassOf [
      rdf:type owl:Restriction ;
      owl:maxCardinality "1"^^xsd:nonNegativeInteger ;
      owl:onProperty ghm:hasNumberOfLeavesPerStem ;
    ] ;
  rdfs:subClassOf [
      rdf:type owl:Restriction ;
      owl:maxCardinality "1"^^xsd:nonNegativeInteger ;
      owl:onProperty ghm:hasPlantNumber ;
    ] ;
  rdfs:subClassOf [
      rdf:type owl:Restriction ;
      owl:maxCardinality "1"^^xsd:nonNegativeInteger ;
      owl:onProperty ghm:hasStemThickness ;
    ] ;
.
ghm:PlantGrowthMeasurement
  rdf:type owl:Class ;
  rdfs:comment "This represents a measurement of the individual growth of a set of plants as well as some general parameters over the entire set, such as average length or color. " ;
  rdfs:label "Plant growth measurement" ;
  rdfs:subClassOf owl:Thing ;
  rdfs:subClassOf [
      rdf:type owl:Restriction ;
      owl:cardinality "1"^^xsd:nonNegativeInteger ;
      owl:onProperty ghm:hasAverageLength ;
    ] ;
  rdfs:subClassOf [
      rdf:type owl:Restriction ;
      owl:cardinality "1"^^xsd:nonNegativeInteger ;
      owl:onProperty ghm:hasAverageNumberOfLeavesPerStem ;
    ] ;
  rdfs:subClassOf [
      rdf:type owl:Restriction ;
      owl:cardinality "1"^^xsd:nonNegativeInteger ;
      owl:onProperty ghm:hasAverageStemThickness ;
    ] ;
  rdfs:subClassOf [
      rdf:type owl:Restriction ;
      owl:cardinality "1"^^xsd:nonNegativeInteger ;
      owl:onProperty ghm:hasDate ;
    ] ;
  rdfs:subClassOf [
      rdf:type owl:Restriction ;
      owl:cardinality "1"^^xsd:nonNegativeInteger ;
      owl:onProperty ghm:hasLeafColor ;
    ] ;
  rdfs:subClassOf [
      rdf:type owl:Restriction ;
      owl:cardinality "1"^^xsd:nonNegativeInteger ;
      owl:onProperty ghm:hasRootColor ;
    ] ;
  rdfs:subClassOf [
      rdf:type owl:Restriction ;
      owl:cardinality "1"^^xsd:nonNegativeInteger ;
      owl:onProperty ghm:hasRootDevelopment ;
    ] ;
  rdfs:subClassOf [
      rdf:type owl:Restriction ;
      owl:cardinality "1"^^xsd:nonNegativeInteger ;
      owl:onProperty ghm:hasUniformity ;
    ] ;
  rdfs:subClassOf [
      rdf:type owl:Restriction ;
      owl:onClass ghm:Block ;
      owl:onProperty ghm:isMeasuredInBlock ;
      owl:qualifiedCardinality "1"^^xsd:nonNegativeInteger ;
    ] ;
  rdfs:subClassOf [
      rdf:type owl:Restriction ;
      owl:onProperty ghm:hasPlantGrowth ;
      owl:someValuesFrom ghm:PlantGrowth ;
    ] ;
.
ghm:System
  rdf:type owl:Class ;
  rdfs:label "System" ;
  rdfs:subClassOf owl:Thing ;
.
ghm:Trait
  rdf:type owl:Class ;
  rdfs:comment "A trait is a characteristic of an individual plant or a group of plants that can be observed and that results from the expression of its genes and their interaction with the environment." ;
  rdfs:comment "Examples of a trait are: fruit shape, seed color, stem diameter, seed length, ...." ;
  rdfs:label "Trait" ;
  rdfs:subClassOf owl:Thing ;
.
ghm:Valve
  rdf:type owl:Class ;
  rdfs:label "Valve" ;
  rdfs:subClassOf owl:Thing ;
.
ghm:WaterAnalysis
  rdf:type owl:Class ;
  rdfs:comment "This class represents analysis on nutritions in a sample of water that is used to irrigate plants in a greenhouse" ;
  rdfs:label "Water analysis" ;
  rdfs:subClassOf owl:Thing ;
  rdfs:subClassOf [
      rdf:type owl:Restriction ;
      owl:cardinality "1"^^xsd:nonNegativeInteger ;
      owl:onProperty ghm:hasDate ;
    ] ;
  rdfs:subClassOf [
      rdf:type owl:Restriction ;
      owl:cardinality "1"^^xsd:nonNegativeInteger ;
      owl:onProperty ghm:hasNutritionRecipe ;
    ] ;
  rdfs:subClassOf [
      rdf:type owl:Restriction ;
      owl:cardinality "1"^^xsd:nonNegativeInteger ;
      owl:onProperty ghm:hasSampleName ;
    ] ;
  rdfs:subClassOf [
      rdf:type owl:Restriction ;
      owl:cardinality "1"^^xsd:nonNegativeInteger ;
      owl:onProperty ghm:hasWeekDay ;
    ] ;
  rdfs:subClassOf [
      rdf:type owl:Restriction ;
      owl:cardinality "1"^^xsd:nonNegativeInteger ;
      owl:onProperty ghm:hasWeekNumber ;
    ] ;
  rdfs:subClassOf [
      rdf:type owl:Restriction ;
      owl:onClass ghm:NutritionLevel ;
      owl:onProperty ghm:hasNutritionLevel ;
      owl:qualifiedCardinality "1"^^xsd:nonNegativeInteger ;
    ] ;
.
ghm:WaterStorageSystem
  rdf:type owl:Class ;
  rdfs:label "Water storage system" ;
  rdfs:subClassOf ghm:WaterSystem ;
.
ghm:WaterSystem
  rdf:type owl:Class ;
  rdfs:comment "This class represents the systems in the greenhouse that deal with water. This includes the infrastructure of the systems as well as the management functionality." ;
  rdfs:label "Water system" ;
  rdfs:subClassOf ghm:System ;
.
ghm:Zone
  rdf:type owl:Class ;
  rdfs:comment "A zone is an area in which the same irrigation and fertilization strategy is applied" ;
  rdfs:label "Zone" ;
  rdfs:subClassOf owl:Thing ;
  rdfs:subClassOf [
      rdf:type owl:Restriction ;
      owl:onProperty ghm:contains ;
      owl:someValuesFrom ghm:IrrigationValve ;
    ] ;
.
ghm:builds
  rdf:type owl:ObjectProperty ;
  rdfs:domain ghm:Builder ;
  rdfs:label "builds" ;
  rdfs:range ghm:Greenhouse ;
  owl:inverseOf ghm:isBuildBy ;
.
ghm:contains
  rdf:type owl:ObjectProperty ;
  rdfs:label "contains" ;
.
ghm:containsBlocks
  rdf:type owl:ObjectProperty ;
  rdfs:domain ghm:Greenhouse ;
  rdfs:label "contains blocks" ;
  rdfs:range ghm:Block ;
  rdfs:subPropertyOf ghm:contains ;
.
ghm:grows
  rdf:type owl:ObjectProperty ;
  rdfs:domain ghm:Grower ;
  rdfs:label "grows" ;
  rdfs:range ghm:Crop ;
  owl:inverseOf ghm:isGrownBy ;
.
ghm:hasAl_level
  rdf:type owl:DatatypeProperty ;
  rdfs:comment "This is the level of aluminium in a sample of water measured in µmol/l" ;
  rdfs:label "has al level" ;
  rdfs:range xsd:float ;
.
ghm:hasAverageLength
  rdf:type owl:DatatypeProperty ;
  rdfs:comment "The average length of all the plants in a measurement in centimeters" ;
  rdfs:domain ghm:PlantGrowthMeasurement ;
  rdfs:label "Average length" ;
  rdfs:range xsd:integer ;
.
ghm:hasAverageNumberOfLeavesPerStem
  rdf:type owl:DatatypeProperty ;
  rdfs:comment "The average number of leaves per stem of all the plants in a measurement" ;
  rdfs:domain ghm:PlantGrowthMeasurement ;
  rdfs:label "has average number of leaves per stem" ;
  rdfs:range xsd:integer ;
.
ghm:hasAverageStemThickness
  rdf:type owl:DatatypeProperty ;
  rdfs:comment "The average thickness of the stem of all plants in a measurement in centimeters with 2 decimals measured 5 centimeters below the knot of the plant" ;
  rdfs:domain ghm:PlantGrowthMeasurement ;
  rdfs:label "has average stem thickness" ;
  rdfs:range xsd:float ;
.
ghm:hasB_level
  rdf:type owl:DatatypeProperty ;
  rdfs:comment "This is the level of boron in a sample of water measured in µmol/l" ;
  rdfs:label "has B level" ;
  rdfs:range xsd:float ;
.
ghm:hasBlockIdentifier
  rdf:type owl:DatatypeProperty ;
  rdfs:comment "Each block has a unique identifier in the greenhouse or compartment in the greenhouse" ;
  rdfs:label "has block identifier" ;
  rdfs:range xsd:string ;
.
ghm:hasCa_level
  rdf:type owl:DatatypeProperty ;
  rdfs:comment "This is the level of calcium in a sample of water measured in mmol/l" ;
  rdfs:label "has ca level" ;
  rdfs:range xsd:float ;
.
ghm:hasCl_level
  rdf:type owl:DatatypeProperty ;
  rdfs:comment "This is the level of chloride in a sample of water measured in mmol/l" ;
  rdfs:label "has cl level" ;
  rdfs:range xsd:float ;
.
ghm:hasCu_level
  rdf:type owl:DatatypeProperty ;
  rdfs:comment "This is the level of copper in a sample of water measured in µmol/l" ;
  rdfs:label "has cu level" ;
  rdfs:range xsd:float ;
.
ghm:hasDate
  rdf:type owl:DatatypeProperty ;
  rdfs:comment "The date at which a measurement in the greenhouse has been executed, e.g. on the growth of a plant, the quality of the water etc." ;
  rdfs:label "has date" ;
  rdfs:range xsd:date ;
.
ghm:hasEC
  rdf:type owl:DatatypeProperty ;
  rdfs:comment "This is the electrical conductivity of a sample of water measured in milliSiemens per centimeter (mS/cm)" ;
  rdfs:label "has EC" ;
  rdfs:range xsd:float ;
.
ghm:hasFe_level
  rdf:type owl:DatatypeProperty ;
  rdfs:comment "This is the level of iron in a sample of water measured in µmol/l" ;
  rdfs:label "has fe level" ;
  rdfs:range xsd:float ;
.
ghm:hasFlowerConstruction
  rdf:type owl:DatatypeProperty ;
  rdfs:comment "The preception of the flower construction of a plant as a number between 1 and 10 from bad to good" ;
  rdfs:domain ghm:PlantGrowthMeasurement ;
  rdfs:label "has flower construction" ;
  rdfs:range xsd:integer ;
.
ghm:hasHCO3_level
  rdf:type owl:DatatypeProperty ;
  rdfs:comment "This is the level of bicarbonate in a sample of water measured in mmol/l" ;
  rdfs:label "has HCO3 level" ;
  rdfs:range xsd:float ;
.
ghm:hasK_Ca_ratio
  rdf:type owl:DatatypeProperty ;
  rdfs:comment "This is the ratio between the levels of kalium and calcium in a sample of water" ;
  rdfs:label "has k Ca ratio" ;
  rdfs:range xsd:float ;
.
ghm:hasK_level
  rdf:type owl:DatatypeProperty ;
  rdfs:comment "This is the level of kalium in a sample of water measured in mmol/l" ;
  rdfs:label "has k level" ;
  rdfs:range xsd:float ;
.
ghm:hasLeafColor
  rdf:type owl:DatatypeProperty ;
  rdfs:comment "The preception of the greenness of the leafs of a plant as a number between 1 and 10 from yellow to dark green" ;
  rdfs:domain ghm:PlantGrowthMeasurement ;
  rdfs:label "has leaf color" ;
  rdfs:range xsd:integer ;
.
ghm:hasLength
  rdf:type owl:DatatypeProperty ;
  rdfs:comment "The length of a plant in centimeters" ;
  rdfs:domain ghm:PlantGrowth ;
  rdfs:label "Length" ;
  rdfs:range xsd:integer ;
.
ghm:hasMg_level
  rdf:type owl:DatatypeProperty ;
  rdfs:comment "This is the level of magnesium in a sample of water measured in mmol/l" ;
  rdfs:label "has mg level" ;
  rdfs:range xsd:float ;
.
ghm:hasMn_level
  rdf:type owl:DatatypeProperty ;
  rdfs:comment "This is the level of manganese in a sample of water measured in µmol/l" ;
  rdfs:label "has k level" ;
  rdfs:range xsd:float ;
.
ghm:hasMo_level
  rdf:type owl:DatatypeProperty ;
  rdfs:comment "This is the level of molybdenum in a sample of water measured in µmol/l" ;
  rdfs:label "has mo level" ;
  rdfs:range xsd:float ;
.
ghm:hasNH4_level
  rdf:type owl:DatatypeProperty ;
  rdfs:comment "This is the level of ammonium in a sample of water measured in mmol/l" ;
  rdfs:label "has NH4 level" ;
  rdfs:range xsd:float ;
.
ghm:hasNO3_level
  rdf:type owl:DatatypeProperty ;
  rdfs:comment "This is the level of nitrate in a sample of water measured in mmol/l" ;
  rdfs:label "has NO3 level" ;
  rdfs:range xsd:float ;
.
ghm:hasN_level
  rdf:type owl:DatatypeProperty ;
  rdfs:comment "This is the level of nitrogen as part of nitrate in a sample of a fluid measured in mmol/l" ;
  rdfs:label "has N level" ;
  rdfs:range xsd:float ;
.
ghm:hasN_total_level
  rdf:type owl:DatatypeProperty ;
  rdfs:comment "This is the total level of nitrogen in a sample of a fluid measured in mmol/l" ;
  rdfs:label "has N total level" ;
  rdfs:range xsd:float ;
.
ghm:hasNa_level
  rdf:type owl:DatatypeProperty ;
  rdfs:comment "This is the level of natrium in a sample of water measured in mmol/l" ;
  rdfs:label "has na level" ;
  rdfs:range xsd:float ;
.
ghm:hasName
  rdf:type owl:DatatypeProperty ;
  rdfs:comment "This is the property that assigns a name to a class" ;
  rdfs:label "has name" ;
  rdfs:range xsd:integer ;
  rdfs:range xsd:string ;
.
ghm:hasNumberOfLeavesPerStem
  rdf:type owl:DatatypeProperty ;
  rdfs:comment "The number of leaves per stem of the plant" ;
  rdfs:domain ghm:PlantGrowth ;
  rdfs:label "has number of leaves per stem" ;
  rdfs:range xsd:integer ;
.
ghm:hasNutritionLevel
  rdf:type owl:ObjectProperty ;
  rdfs:domain ghm:WaterAnalysis ;
  rdfs:label "has nutrition level" ;
  rdfs:range ghm:NutritionLevel ;
.
ghm:hasNutritionRecipe
  rdf:type owl:DatatypeProperty ;
  rdfs:comment "This is the name of the nutrition recipe that is used to irrigate plants in a greenhouse" ;
  rdfs:label "has nutrition recipe" ;
  rdfs:range xsd:string ;
.
ghm:hasP_level
  rdf:type owl:DatatypeProperty ;
  rdfs:comment "This is the level of phosphorus in a sample of water measured in mmol/l" ;
  rdfs:label "has P level" ;
  rdfs:range xsd:float ;
.
ghm:hasPlantGrowth
  rdf:type owl:ObjectProperty ;
  rdfs:domain ghm:PlantGrowthMeasurement ;
  rdfs:label "has plant growth" ;
  rdfs:range ghm:PlantGrowth ;
.
ghm:hasPlantNumber
  rdf:type owl:DatatypeProperty ;
  rdfs:comment "The number of the plant as part of a measurement performed on its growth" ;
  rdfs:domain ghm:PlantGrowth ;
  rdfs:label "has plant number" ;
  rdfs:range xsd:integer ;
.
ghm:hasRootColor
  rdf:type owl:DatatypeProperty ;
  rdfs:comment "The preception of the level of development of the root of a plant as a number between 1 and 10 from bad to good" ;
  rdfs:domain ghm:PlantGrowthMeasurement ;
  rdfs:label "has root color" ;
  rdfs:range xsd:integer ;
.
ghm:hasRootDevelopment
  rdf:type owl:DatatypeProperty ;
  rdfs:comment "The preception of the level of development of the root of a plant as a number between 1 and 10 from bad to good" ;
  rdfs:domain ghm:PlantGrowthMeasurement ;
  rdfs:label "has root development" ;
  rdfs:range xsd:integer ;
.
ghm:hasS_level
  rdf:type owl:DatatypeProperty ;
  rdfs:comment "This is the level of sulfur in a sample of water measured in mmol/l" ;
  rdfs:label "has S level" ;
  rdfs:range xsd:float ;
.
ghm:hasSampleName
  rdf:type owl:DatatypeProperty ;
  rdfs:comment "This is the name of a sample for analysis on nutritions in water that is used to irrigate plants in a greenhouse" ;
  rdfs:label "has sample name" ;
  rdfs:range xsd:string ;
.
ghm:hasSi_level
  rdf:type owl:DatatypeProperty ;
  rdfs:comment "This is the level of silicon in a sample of water measured in mmol/l" ;
  rdfs:label "has si level" ;
  rdfs:range xsd:float ;
.
ghm:hasStemThickness
  rdf:type owl:DatatypeProperty ;
  rdfs:comment "The thickness of the stem in centimeters with 2 decimals measured 5 centimeters below the knot of the plant" ;
  rdfs:domain ghm:PlantGrowth ;
  rdfs:label "has stem thickness" ;
  rdfs:range xsd:float ;
.
ghm:hasSugar_concentration
  rdf:type owl:DatatypeProperty ;
  rdfs:comment "This is the concentration of sugar in a sample of a fluid measured in a percentage" ;
  rdfs:label "has sugar concentration" ;
  rdfs:range xsd:float ;
.
ghm:hasUniformity
  rdf:type owl:DatatypeProperty ;
  rdfs:comment "The preception of the uniformity of a plant as a number between 1 and 10 from bad to good" ;
  rdfs:domain ghm:PlantGrowthMeasurement ;
  rdfs:label "has uniformity" ;
  rdfs:range xsd:integer ;
.
ghm:hasWeekDay
  rdf:type owl:DatatypeProperty ;
  rdfs:comment "The name of the day in the week in which a measurement in the greenhouse has been executed" ;
  rdfs:label "has week day" ;
  rdfs:range xsd:gDay ;
.
ghm:hasWeekNumber
  rdf:type owl:DatatypeProperty ;
  rdfs:comment "The calendar number of the week in which a measurement in the greenhouse has been executed" ;
  rdfs:label "has week number" ;
  rdfs:range xsd:integer ;
.
ghm:hasZn_level
  rdf:type owl:DatatypeProperty ;
  rdfs:comment "This is the level of zinc in a sample of water measured in µmol/l" ;
  rdfs:label "has zn level" ;
  rdfs:range xsd:float ;
.
ghm:haspH
  rdf:type owl:DatatypeProperty ;
  rdfs:label "hasp HLevel" ;
  rdfs:range xsd:float ;
.
ghm:isBuildBy
  rdf:type owl:ObjectProperty ;
  rdfs:domain ghm:Greenhouse ;
  rdfs:label "is build by" ;
  rdfs:range ghm:Builder ;
  owl:inverseOf ghm:builds ;
.
ghm:isGrownBy
  rdf:type owl:ObjectProperty ;
  rdfs:domain ghm:Crop ;
  rdfs:label "is grown by" ;
  rdfs:range ghm:Grower ;
  owl:inverseOf ghm:grows ;
.
ghm:isGrownIn
  rdf:type owl:ObjectProperty ;
  rdfs:domain ghm:Crop ;
  rdfs:label "is grown in" ;
  rdfs:range ghm:Greenhouse ;
.
ghm:isMeasuredInBlock
  rdf:type owl:ObjectProperty ;
  rdfs:domain ghm:PlantGrowthMeasurement ;
  rdfs:label "is located in block" ;
  rdfs:range ghm:Block ;
.
ghm:isOperatedBy
  rdf:type owl:ObjectProperty ;
  rdfs:domain ghm:Greenhouse ;
  rdfs:label "is operated by" ;
  rdfs:range ghm:Grower ;
.
ghm:ofCrop
  rdf:type owl:ObjectProperty ;
  rdfs:comment "This property represents the relation between an analysis and the crop that is analyzed" ;
  rdfs:domain ghm:LeafJuiceAnalysis ;
  rdfs:label "of crop" ;
  rdfs:range ghm:Crop ;
.
ghm:ofCropPart
  rdf:type owl:DatatypeProperty ;
  rdfs:comment "This property represents the relation between an analysis and the part of the crop that is analyzed, e.g. young or old" ;
  rdfs:domain ghm:LeafJuiceAnalysis ;
  rdfs:label "of crop" ;
  rdfs:range xsd:string ;
.
ghm:operates
  rdf:type owl:ObjectProperty ;
  rdfs:domain ghm:Grower ;
  rdfs:label "operates" ;
  rdfs:range ghm:Greenhouse ;
  owl:inverseOf ghm:isOperatedBy ;
.
ghm:snoeptomaatje
  rdf:type ghm:Crop ;
  rdfs:label "snoeptomaatje" ;
.
