@prefix : <https://www.tno.nl/agrifood/ontology/greenhouse-model/> .
@prefix um: <http://www.ontology-of-units-of-measure.org/resource/om-2/> .
@prefix ghm: <https://www.tno.nl/agrifood/ontology/greenhouse-model/> .
@prefix owl: <http://www.w3.org/2002/07/owl#> .
@prefix rdf: <http://www.w3.org/1999/02/22-rdf-syntax-ns#> .
@prefix xml: <http://www.w3.org/XML/1998/namespace> .
@prefix xsd: <http://www.w3.org/2001/XMLSchema#> .
@prefix rdfs: <http://www.w3.org/2000/01/rdf-schema#> .
@prefix spin: <http://spinrdf.org/spin#> .
@prefix MathM: <http://www.w3.org/1998/Math/MathML> .
@base <https://www.tno.nl/agrifood/ontology/greenhouse-model/> .

<https://www.tno.nl/agrifood/ontology/greenhouse-model/> rdf:type owl:Ontology ;
                                                          owl:imports <https://raw.githubusercontent.com/HajoRijgersberg/OM/master/om-2.0.rdf> ;
                                                          spin:imports <http://topbraid.org/spin/owlrl-all> .

#################################################################
#    Annotation properties
#################################################################

###  http://spinrdf.org/spin#imports
spin:imports rdf:type owl:AnnotationProperty .


#################################################################
#    Datatypes
#################################################################

###  http://www.w3.org/2001/XMLSchema#date
xsd:date rdf:type rdfs:Datatype .


###  http://www.w3.org/2001/XMLSchema#gDay
xsd:gDay rdf:type rdfs:Datatype .


#################################################################
#    Object Properties
#################################################################

###  https://www.tno.nl/agrifood/ontology/greenhouse-model/builds
ghm:builds rdf:type owl:ObjectProperty ;
           owl:inverseOf ghm:isBuildBy ;
           rdfs:domain ghm:Builder ;
           rdfs:range ghm:Greenhouse ;
           rdfs:label "builds" .


###  https://www.tno.nl/agrifood/ontology/greenhouse-model/contains
ghm:contains rdf:type owl:ObjectProperty ;
             rdfs:label "contains" .


###  https://www.tno.nl/agrifood/ontology/greenhouse-model/containsBlocks
ghm:containsBlocks rdf:type owl:ObjectProperty ;
                   rdfs:subPropertyOf ghm:contains ;
                   rdfs:domain ghm:Greenhouse ;
                   rdfs:range ghm:Block ;
                   rdfs:label "contains blocks" .


###  https://www.tno.nl/agrifood/ontology/greenhouse-model/grows
ghm:grows rdf:type owl:ObjectProperty ;
          owl:inverseOf ghm:isGrownBy ;
          rdfs:domain ghm:Grower ;
          rdfs:range ghm:Crop ;
          rdfs:label "grows" .


###  https://www.tno.nl/agrifood/ontology/greenhouse-model/hasNutritionLevel
ghm:hasNutritionLevel rdf:type owl:ObjectProperty ;
                      rdfs:domain ghm:WaterAnalysis ;
                      rdfs:range ghm:NutritionLevel ;
                      rdfs:label "has nutrition level" .


###  https://www.tno.nl/agrifood/ontology/greenhouse-model/hasPlantGrowth
ghm:hasPlantGrowth rdf:type owl:ObjectProperty ;
                   rdfs:domain ghm:PlantGrowthMeasurement ;
                   rdfs:range ghm:PlantGrowth ;
                   rdfs:label "has plant growth" .


###  https://www.tno.nl/agrifood/ontology/greenhouse-model/isBuildBy
ghm:isBuildBy rdf:type owl:ObjectProperty ;
              rdfs:domain ghm:Greenhouse ;
              rdfs:range ghm:Builder ;
              rdfs:label "is build by" .


###  https://www.tno.nl/agrifood/ontology/greenhouse-model/isGrownBy
ghm:isGrownBy rdf:type owl:ObjectProperty ;
              rdfs:domain ghm:Crop ;
              rdfs:range ghm:Grower ;
              rdfs:label "is grown by" .


###  https://www.tno.nl/agrifood/ontology/greenhouse-model/isGrownIn
ghm:isGrownIn rdf:type owl:ObjectProperty ;
              rdfs:domain ghm:Crop ;
              rdfs:range ghm:Greenhouse ;
              rdfs:label "is grown in" .


###  https://www.tno.nl/agrifood/ontology/greenhouse-model/isMeasuredInBlock
ghm:isMeasuredInBlock rdf:type owl:ObjectProperty ;
                      rdfs:domain ghm:PlantGrowthMeasurement ;
                      rdfs:range ghm:Block ;
                      rdfs:label "is located in block" .


###  https://www.tno.nl/agrifood/ontology/greenhouse-model/isOperatedBy
ghm:isOperatedBy rdf:type owl:ObjectProperty ;
                 owl:inverseOf ghm:operates ;
                 rdfs:domain ghm:Greenhouse ;
                 rdfs:range ghm:Grower ;
                 rdfs:label "is operated by" .


###  https://www.tno.nl/agrifood/ontology/greenhouse-model/ofCrop
ghm:ofCrop rdf:type owl:ObjectProperty ;
           rdfs:domain ghm:LeafJuiceAnalysis ;
           rdfs:range ghm:Crop ;
           rdfs:comment "This property represents the relation between an analysis and the crop that is analyzed" ;
           rdfs:label "of crop" .


###  https://www.tno.nl/agrifood/ontology/greenhouse-model/operates
ghm:operates rdf:type owl:ObjectProperty ;
             rdfs:domain ghm:Grower ;
             rdfs:range ghm:Greenhouse ;
             rdfs:label "operates" .


#################################################################
#    Data properties
#################################################################

###  https://www.tno.nl/agrifood/ontology/greenhouse-model/hasAl_level
ghm:hasAl_level rdf:type owl:DatatypeProperty ;
                rdfs:range xsd:float ;
                rdfs:comment "This is the level of aluminium in a sample of water measured in µmol/l" ;
                rdfs:label "has al level" .


###  https://www.tno.nl/agrifood/ontology/greenhouse-model/hasAverageLength
ghm:hasAverageLength rdf:type owl:DatatypeProperty ;
                     rdfs:domain ghm:PlantGrowthMeasurement ;
                     rdfs:range xsd:integer ;
                     rdfs:comment "The average length of all the plants in a measurement in centimeters" ;
                     rdfs:label "Average length" .


###  https://www.tno.nl/agrifood/ontology/greenhouse-model/hasAverageNumberOfLeavesPerStem
ghm:hasAverageNumberOfLeavesPerStem rdf:type owl:DatatypeProperty ;
                                    rdfs:domain ghm:PlantGrowthMeasurement ;
                                    rdfs:range xsd:integer ;
                                    rdfs:comment "The average number of leaves per stem of all the plants in a measurement" ;
                                    rdfs:label "has average number of leaves per stem" .


###  https://www.tno.nl/agrifood/ontology/greenhouse-model/hasAverageStemThickness
ghm:hasAverageStemThickness rdf:type owl:DatatypeProperty ;
                            rdfs:domain ghm:PlantGrowthMeasurement ;
                            rdfs:range xsd:float ;
                            rdfs:comment "The average thickness of the stem of all plants in a measurement in centimeters with 2 decimals measured 5 centimeters below the knot of the plant" ;
                            rdfs:label "has average stem thickness" .


###  https://www.tno.nl/agrifood/ontology/greenhouse-model/hasB_level
ghm:hasB_level rdf:type owl:DatatypeProperty ;
               rdfs:range xsd:float ;
               rdfs:comment "This is the level of boron in a sample of water measured in µmol/l" ;
               rdfs:label "has B level" .


###  https://www.tno.nl/agrifood/ontology/greenhouse-model/hasBlockIdentifier
ghm:hasBlockIdentifier rdf:type owl:DatatypeProperty ;
                       rdfs:range xsd:string ;
                       rdfs:comment "Each block has a unique identifier in the greenhouse or compartment in the greenhouse" ;
                       rdfs:label "has block identifier" .


###  https://www.tno.nl/agrifood/ontology/greenhouse-model/hasCa_level
ghm:hasCa_level rdf:type owl:DatatypeProperty ;
                rdfs:range xsd:float ;
                rdfs:comment "This is the level of calcium in a sample of water measured in mmol/l" ;
                rdfs:label "has ca level" .


###  https://www.tno.nl/agrifood/ontology/greenhouse-model/hasCl_level
ghm:hasCl_level rdf:type owl:DatatypeProperty ;
                rdfs:range xsd:float ;
                rdfs:comment "This is the level of chloride in a sample of water measured in mmol/l" ;
                rdfs:label "has cl level" .


###  https://www.tno.nl/agrifood/ontology/greenhouse-model/hasCu_level
ghm:hasCu_level rdf:type owl:DatatypeProperty ;
                rdfs:range xsd:float ;
                rdfs:comment "This is the level of copper in a sample of water measured in µmol/l" ;
                rdfs:label "has cu level" .


###  https://www.tno.nl/agrifood/ontology/greenhouse-model/hasDate
ghm:hasDate rdf:type owl:DatatypeProperty ;
            rdfs:range xsd:date ;
            rdfs:comment "The date at which a measurement in the greenhouse has been executed, e.g. on the growth of a plant, the quality of the water etc." ;
            rdfs:label "has date" .


###  https://www.tno.nl/agrifood/ontology/greenhouse-model/hasEC
ghm:hasEC rdf:type owl:DatatypeProperty ;
          rdfs:range xsd:float ;
          rdfs:comment "This is the electrical conductivity of a sample of water measured in milliSiemens per centimeter (mS/cm)" ;
          rdfs:label "has EC" .


###  https://www.tno.nl/agrifood/ontology/greenhouse-model/hasFe_level
ghm:hasFe_level rdf:type owl:DatatypeProperty ;
                rdfs:range xsd:float ;
                rdfs:comment "This is the level of iron in a sample of water measured in µmol/l" ;
                rdfs:label "has fe level" .


###  https://www.tno.nl/agrifood/ontology/greenhouse-model/hasFlowerConstruction
ghm:hasFlowerConstruction rdf:type owl:DatatypeProperty ;
                          rdfs:domain ghm:PlantGrowthMeasurement ;
                          rdfs:range xsd:integer ;
                          rdfs:comment "The preception of the flower construction of a plant as a number between 1 and 10 from bad to good" ;
                          rdfs:label "has flower construction" .


###  https://www.tno.nl/agrifood/ontology/greenhouse-model/hasHCO3_level
ghm:hasHCO3_level rdf:type owl:DatatypeProperty ;
                  rdfs:range xsd:float ;
                  rdfs:comment "This is the level of bicarbonate in a sample of water measured in mmol/l" ;
                  rdfs:label "has HCO3 level" .


###  https://www.tno.nl/agrifood/ontology/greenhouse-model/hasK_Ca_ratio
ghm:hasK_Ca_ratio rdf:type owl:DatatypeProperty ;
                  rdfs:range xsd:float ;
                  rdfs:comment "This is the ratio between the levels of kalium and calcium in a sample of water" ;
                  rdfs:label "has k Ca ratio" .


###  https://www.tno.nl/agrifood/ontology/greenhouse-model/hasK_level
ghm:hasK_level rdf:type owl:DatatypeProperty ;
               rdfs:range xsd:float ;
               rdfs:comment "This is the level of kalium in a sample of water measured in mmol/l" ;
               rdfs:label "has k level" .


###  https://www.tno.nl/agrifood/ontology/greenhouse-model/hasLeafColor
ghm:hasLeafColor rdf:type owl:DatatypeProperty ;
                 rdfs:domain ghm:PlantGrowthMeasurement ;
                 rdfs:range xsd:integer ;
                 rdfs:comment "The preception of the greenness of the leafs of a plant as a number between 1 and 10 from yellow to dark green" ;
                 rdfs:label "has leaf color" .


###  https://www.tno.nl/agrifood/ontology/greenhouse-model/hasLength
ghm:hasLength rdf:type owl:DatatypeProperty ;
              rdfs:domain ghm:PlantGrowth ;
              rdfs:range xsd:integer ;
              rdfs:comment "The length of a plant in centimeters" ;
              rdfs:label "Length" .


###  https://www.tno.nl/agrifood/ontology/greenhouse-model/hasMg_level
ghm:hasMg_level rdf:type owl:DatatypeProperty ;
                rdfs:range xsd:float ;
                rdfs:comment "This is the level of magnesium in a sample of water measured in mmol/l" ;
                rdfs:label "has mg level" .


###  https://www.tno.nl/agrifood/ontology/greenhouse-model/hasMn_level
ghm:hasMn_level rdf:type owl:DatatypeProperty ;
                rdfs:range xsd:float ;
                rdfs:comment "This is the level of manganese in a sample of water measured in µmol/l" ;
                rdfs:label "has k level" .


###  https://www.tno.nl/agrifood/ontology/greenhouse-model/hasMo_level
ghm:hasMo_level rdf:type owl:DatatypeProperty ;
                rdfs:range xsd:float ;
                rdfs:comment "This is the level of molybdenum in a sample of water measured in µmol/l" ;
                rdfs:label "has mo level" .


###  https://www.tno.nl/agrifood/ontology/greenhouse-model/hasNH4_level
ghm:hasNH4_level rdf:type owl:DatatypeProperty ;
                 rdfs:range xsd:float ;
                 rdfs:comment "This is the level of ammonium in a sample of water measured in mmol/l" ;
                 rdfs:label "has NH4 level" .


###  https://www.tno.nl/agrifood/ontology/greenhouse-model/hasNO3_level
ghm:hasNO3_level rdf:type owl:DatatypeProperty ;
                 rdfs:range xsd:float ;
                 rdfs:comment "This is the level of nitrate in a sample of water measured in mmol/l" ;
                 rdfs:label "has NO3 level" .


###  https://www.tno.nl/agrifood/ontology/greenhouse-model/hasN_level
ghm:hasN_level rdf:type owl:DatatypeProperty ;
               rdfs:range xsd:float ;
               rdfs:comment "This is the level of nitrogen as part of nitrate in a sample of a fluid measured in mmol/l" ;
               rdfs:label "has N level" .


###  https://www.tno.nl/agrifood/ontology/greenhouse-model/hasN_total_level
ghm:hasN_total_level rdf:type owl:DatatypeProperty ;
                     rdfs:range xsd:float ;
                     rdfs:comment "This is the total level of nitrogen in a sample of a fluid measured in mmol/l" ;
                     rdfs:label "has N total level" .


###  https://www.tno.nl/agrifood/ontology/greenhouse-model/hasNa_level
ghm:hasNa_level rdf:type owl:DatatypeProperty ;
                rdfs:range xsd:float ;
                rdfs:comment "This is the level of natrium in a sample of water measured in mmol/l" ;
                rdfs:label "has na level" .


###  https://www.tno.nl/agrifood/ontology/greenhouse-model/hasName
ghm:hasName rdf:type owl:DatatypeProperty ;
            rdfs:range xsd:integer ,
                       xsd:string ;
            rdfs:comment "This is the property that assigns a name to a class" ;
            rdfs:label "has name" .


###  https://www.tno.nl/agrifood/ontology/greenhouse-model/hasNumberOfLeavesPerStem
ghm:hasNumberOfLeavesPerStem rdf:type owl:DatatypeProperty ;
                             rdfs:domain ghm:PlantGrowth ;
                             rdfs:range xsd:integer ;
                             rdfs:comment "The number of leaves per stem of the plant" ;
                             rdfs:label "has number of leaves per stem" .


###  https://www.tno.nl/agrifood/ontology/greenhouse-model/hasNutritionRecipe
ghm:hasNutritionRecipe rdf:type owl:DatatypeProperty ;
                       rdfs:range xsd:string ;
                       rdfs:comment "This is the name of the nutrition recipe that is used to irrigate plants in a greenhouse" ;
                       rdfs:label "has nutrition recipe" .


###  https://www.tno.nl/agrifood/ontology/greenhouse-model/hasP_level
ghm:hasP_level rdf:type owl:DatatypeProperty ;
               rdfs:range xsd:float ;
               rdfs:comment "This is the level of phosphorus in a sample of water measured in mmol/l" ;
               rdfs:label "has P level" .


###  https://www.tno.nl/agrifood/ontology/greenhouse-model/hasPlantNumber
ghm:hasPlantNumber rdf:type owl:DatatypeProperty ;
                   rdfs:domain ghm:PlantGrowth ;
                   rdfs:range xsd:integer ;
                   rdfs:comment "The number of the plant as part of a measurement performed on its growth" ;
                   rdfs:label "has plant number" .


###  https://www.tno.nl/agrifood/ontology/greenhouse-model/hasRootColor
ghm:hasRootColor rdf:type owl:DatatypeProperty ;
                 rdfs:domain ghm:PlantGrowthMeasurement ;
                 rdfs:range xsd:integer ;
                 rdfs:comment "The preception of the level of development of the root of a plant as a number between 1 and 10 from bad to good" ;
                 rdfs:label "has root color" .


###  https://www.tno.nl/agrifood/ontology/greenhouse-model/hasRootDevelopment
ghm:hasRootDevelopment rdf:type owl:DatatypeProperty ;
                       rdfs:domain ghm:PlantGrowthMeasurement ;
                       rdfs:range xsd:integer ;
                       rdfs:comment "The preception of the level of development of the root of a plant as a number between 1 and 10 from bad to good" ;
                       rdfs:label "has root development" .


###  https://www.tno.nl/agrifood/ontology/greenhouse-model/hasS_level
ghm:hasS_level rdf:type owl:DatatypeProperty ;
               rdfs:range xsd:float ;
               rdfs:comment "This is the level of sulfur in a sample of water measured in mmol/l" ;
               rdfs:label "has S level" .


###  https://www.tno.nl/agrifood/ontology/greenhouse-model/hasSampleName
ghm:hasSampleName rdf:type owl:DatatypeProperty ;
                  rdfs:range xsd:string ;
                  rdfs:comment "This is the name of a sample for analysis on nutritions in water that is used to irrigate plants in a greenhouse" ;
                  rdfs:label "has sample name" .


###  https://www.tno.nl/agrifood/ontology/greenhouse-model/hasSi_level
ghm:hasSi_level rdf:type owl:DatatypeProperty ;
                rdfs:range xsd:float ;
                rdfs:comment "This is the level of silicon in a sample of water measured in mmol/l" ;
                rdfs:label "has si level" .


###  https://www.tno.nl/agrifood/ontology/greenhouse-model/hasStemThickness
ghm:hasStemThickness rdf:type owl:DatatypeProperty ;
                     rdfs:domain ghm:PlantGrowth ;
                     rdfs:range xsd:float ;
                     rdfs:comment "The thickness of the stem in centimeters with 2 decimals measured 5 centimeters below the knot of the plant" ;
                     rdfs:label "has stem thickness" .


###  https://www.tno.nl/agrifood/ontology/greenhouse-model/hasSugar_concentration
ghm:hasSugar_concentration rdf:type owl:DatatypeProperty ;
                           rdfs:range xsd:float ;
                           rdfs:comment "This is the concentration of sugar in a sample of a fluid measured in a percentage" ;
                           rdfs:label "has sugar concentration" .


###  https://www.tno.nl/agrifood/ontology/greenhouse-model/hasUniformity
ghm:hasUniformity rdf:type owl:DatatypeProperty ;
                  rdfs:domain ghm:PlantGrowthMeasurement ;
                  rdfs:range xsd:integer ;
                  rdfs:comment "The preception of the uniformity of a plant as a number between 1 and 10 from bad to good" ;
                  rdfs:label "has uniformity" .


###  https://www.tno.nl/agrifood/ontology/greenhouse-model/hasWeekDay
ghm:hasWeekDay rdf:type owl:DatatypeProperty ;
               rdfs:range xsd:gDay ;
               rdfs:comment "The name of the day in the week in which a measurement in the greenhouse has been executed" ;
               rdfs:label "has week day" .


###  https://www.tno.nl/agrifood/ontology/greenhouse-model/hasWeekNumber
ghm:hasWeekNumber rdf:type owl:DatatypeProperty ;
                  rdfs:range xsd:integer ;
                  rdfs:comment "The calendar number of the week in which a measurement in the greenhouse has been executed" ;
                  rdfs:label "has week number" .


###  https://www.tno.nl/agrifood/ontology/greenhouse-model/hasZn_level
ghm:hasZn_level rdf:type owl:DatatypeProperty ;
                rdfs:range xsd:float ;
                rdfs:comment "This is the level of zinc in a sample of water measured in µmol/l" ;
                rdfs:label "has zn level" .


###  https://www.tno.nl/agrifood/ontology/greenhouse-model/haspH
ghm:haspH rdf:type owl:DatatypeProperty ;
          rdfs:range xsd:float ;
          rdfs:label "hasp HLevel" .


###  https://www.tno.nl/agrifood/ontology/greenhouse-model/ofCropPart
ghm:ofCropPart rdf:type owl:DatatypeProperty ;
               rdfs:domain ghm:LeafJuiceAnalysis ;
               rdfs:range xsd:string ;
               rdfs:comment "This property represents the relation between an analysis and the part of the crop that is analyzed, e.g. young or old" ;
               rdfs:label "of crop" .


#################################################################
#    Classes
#################################################################

###  http://www.w3.org/2002/07/owl#Thing
owl:Thing rdf:type owl:Class .


###  https://www.tno.nl/agrifood/ontology/greenhouse-model/Block
ghm:Block rdf:type owl:Class ;
          rdfs:subClassOf owl:Thing ,
                          [ rdf:type owl:Restriction ;
                            owl:onProperty ghm:contains ;
                            owl:qualifiedCardinality "1"^^xsd:nonNegativeInteger ;
                            owl:onClass ghm:Crop
                          ] ,
                          [ rdf:type owl:Restriction ;
                            owl:onProperty ghm:hasBlockIdentifier ;
                            owl:cardinality "1"^^xsd:nonNegativeInteger
                          ] ;
          rdfs:comment "A block contains only a single crop (this is a requirement)" ,
                       "A block is part of a compartment in the greenhouse in which the plants are treated equally wrt nutrition, climate etc." ,
                       "Each block has a unique identifier in the greenhouse or compartment in the greenhouse" ,
                       "This class represents blocks that are part of a greenhouse and contain a set of plants" ;
          rdfs:label "Block" .


###  https://www.tno.nl/agrifood/ontology/greenhouse-model/Builder
ghm:Builder rdf:type owl:Class ;
            rdfs:subClassOf owl:Thing ;
            rdfs:comment "This class represents builders that build greenhouses and possibly support growers in their crop management activities" ;
            rdfs:label "Builder" .


###  https://www.tno.nl/agrifood/ontology/greenhouse-model/Compartment
ghm:Compartment rdf:type owl:Class ;
                rdfs:subClassOf owl:Thing ,
                                [ rdf:type owl:Restriction ;
                                  owl:onProperty ghm:contains ;
                                  owl:someValuesFrom ghm:Block
                                ] ,
                                [ rdf:type owl:Restriction ;
                                  owl:onProperty ghm:contains ;
                                  owl:someValuesFrom ghm:Zone
                                ] ;
                rdfs:comment "A compartment is a part of the greenhouse" ,
                             "Each compartment has a unique identifier in the greenhouse" ,
                             "This class represents compartments that are part of a greenhouse and contain a set of plants" ;
                rdfs:label "Block" .


###  https://www.tno.nl/agrifood/ontology/greenhouse-model/Crop
ghm:Crop rdf:type owl:Class ;
         rdfs:subClassOf owl:Thing ,
                         [ rdf:type owl:Restriction ;
                           owl:onProperty ghm:isGrownBy ;
                           owl:someValuesFrom ghm:Grower
                         ] ,
                         [ rdf:type owl:Restriction ;
                           owl:onProperty ghm:isGrownIn ;
                           owl:someValuesFrom ghm:Greenhouse
                         ] ,
                         [ rdf:type owl:Restriction ;
                           owl:onProperty ghm:hasName ;
                           owl:cardinality "1"^^xsd:nonNegativeInteger
                         ] ;
         rdfs:comment "More characteristics of a crop can be defined using the guideline for creating a crop ontology published here: http://www.cropontology.org" ,
                      "This class represents crops that are produced in a greenhouse operated by a grower" ;
         rdfs:label "Crop" .


###  https://www.tno.nl/agrifood/ontology/greenhouse-model/DisinfectionSystem
ghm:DisinfectionSystem rdf:type owl:Class ;
                       rdfs:subClassOf ghm:WaterSystem ;
                       rdfs:label "Disinfection system" .


###  https://www.tno.nl/agrifood/ontology/greenhouse-model/Greenhouse
ghm:Greenhouse rdf:type owl:Class ;
               rdfs:subClassOf owl:Thing ,
                               [ rdf:type owl:Restriction ;
                                 owl:onProperty ghm:contains ;
                                 owl:someValuesFrom ghm:Compartment
                               ] ,
                               [ rdf:type owl:Restriction ;
                                 owl:onProperty ghm:contains ;
                                 owl:someValuesFrom ghm:System
                               ] ,
                               [ rdf:type owl:Restriction ;
                                 owl:onProperty ghm:containsBlocks ;
                                 owl:someValuesFrom ghm:Block
                               ] ,
                               [ rdf:type owl:Restriction ;
                                 owl:onProperty ghm:isBuildBy ;
                                 owl:qualifiedCardinality "1"^^xsd:nonNegativeInteger ;
                                 owl:onClass ghm:Builder
                               ] ,
                               [ rdf:type owl:Restriction ;
                                 owl:onProperty ghm:isOperatedBy ;
                                 owl:qualifiedCardinality "1"^^xsd:nonNegativeInteger ;
                                 owl:onClass ghm:Grower
                               ] ;
               rdfs:comment "This class represents greenhouses in which crop is being grown by a grower" ;
               rdfs:label "Greenhouse" .


###  https://www.tno.nl/agrifood/ontology/greenhouse-model/Grower
ghm:Grower rdf:type owl:Class ;
           rdfs:subClassOf owl:Thing ,
                           [ rdf:type owl:Restriction ;
                             owl:onProperty ghm:grows ;
                             owl:someValuesFrom ghm:Crop
                           ] ;
           rdfs:comment "This class represents growers that operate and possibly own a greenhouse to produce one or more crops as efficient and effective as possible" ;
           rdfs:label "Grower" .


###  https://www.tno.nl/agrifood/ontology/greenhouse-model/IrrigationValve
ghm:IrrigationValve rdf:type owl:Class ;
                    rdfs:subClassOf ghm:Valve ;
                    rdfs:comment "An irrigation valve is a switch that steers the amount of water in a zone" ;
                    rdfs:label "Irrigation valve" .


###  https://www.tno.nl/agrifood/ontology/greenhouse-model/IrrigtationSystem
ghm:IrrigtationSystem rdf:type owl:Class ;
                      rdfs:subClassOf ghm:WaterSystem ;
                      rdfs:label "Irrigtation system" .


###  https://www.tno.nl/agrifood/ontology/greenhouse-model/LeafJuiceAnalysis
ghm:LeafJuiceAnalysis rdf:type owl:Class ;
                      rdfs:subClassOf owl:Thing ,
                                      [ rdf:type owl:Restriction ;
                                        owl:onProperty ghm:ofCrop ;
                                        owl:someValuesFrom ghm:Crop
                                      ] ,
                                      [ rdf:type owl:Restriction ;
                                        owl:onProperty ghm:hasNutritionLevel ;
                                        owl:qualifiedCardinality "1"^^xsd:nonNegativeInteger ;
                                        owl:onClass ghm:NutritionLevel
                                      ] ,
                                      [ rdf:type owl:Restriction ;
                                        owl:onProperty ghm:hasDate ;
                                        owl:cardinality "1"^^xsd:nonNegativeInteger
                                      ] ,
                                      [ rdf:type owl:Restriction ;
                                        owl:onProperty ghm:hasNutritionRecipe ;
                                        owl:cardinality "1"^^xsd:nonNegativeInteger
                                      ] ,
                                      [ rdf:type owl:Restriction ;
                                        owl:onProperty ghm:hasSampleName ;
                                        owl:cardinality "1"^^xsd:nonNegativeInteger
                                      ] ,
                                      [ rdf:type owl:Restriction ;
                                        owl:onProperty ghm:hasWeekNumber ;
                                        owl:cardinality "1"^^xsd:nonNegativeInteger
                                      ] ,
                                      [ rdf:type owl:Restriction ;
                                        owl:onProperty ghm:ofCropPart ;
                                        owl:cardinality "1"^^xsd:nonNegativeInteger
                                      ] ;
                      rdfs:comment "This class represents analysis on nutritions in a sample of leaf juice of plants in a greenhouse" ;
                      rdfs:label "Leaf juice analysis" .


###  https://www.tno.nl/agrifood/ontology/greenhouse-model/NutritionLevel
ghm:NutritionLevel rdf:type owl:Class ;
                   rdfs:subClassOf owl:Thing ,
                                   [ rdf:type owl:Restriction ;
                                     owl:onProperty ghm:hasAl_level ;
                                     owl:cardinality "1"^^xsd:nonNegativeInteger
                                   ] ,
                                   [ rdf:type owl:Restriction ;
                                     owl:onProperty ghm:hasB_level ;
                                     owl:cardinality "1"^^xsd:nonNegativeInteger
                                   ] ,
                                   [ rdf:type owl:Restriction ;
                                     owl:onProperty ghm:hasCa_level ;
                                     owl:cardinality "1"^^xsd:nonNegativeInteger
                                   ] ,
                                   [ rdf:type owl:Restriction ;
                                     owl:onProperty ghm:hasCl_level ;
                                     owl:cardinality "1"^^xsd:nonNegativeInteger
                                   ] ,
                                   [ rdf:type owl:Restriction ;
                                     owl:onProperty ghm:hasCu_level ;
                                     owl:cardinality "1"^^xsd:nonNegativeInteger
                                   ] ,
                                   [ rdf:type owl:Restriction ;
                                     owl:onProperty ghm:hasEC ;
                                     owl:cardinality "1"^^xsd:nonNegativeInteger
                                   ] ,
                                   [ rdf:type owl:Restriction ;
                                     owl:onProperty ghm:hasFe_level ;
                                     owl:cardinality "1"^^xsd:nonNegativeInteger
                                   ] ,
                                   [ rdf:type owl:Restriction ;
                                     owl:onProperty ghm:hasHCO3_level ;
                                     owl:cardinality "1"^^xsd:nonNegativeInteger
                                   ] ,
                                   [ rdf:type owl:Restriction ;
                                     owl:onProperty ghm:hasK_Ca_ratio ;
                                     owl:cardinality "1"^^xsd:nonNegativeInteger
                                   ] ,
                                   [ rdf:type owl:Restriction ;
                                     owl:onProperty ghm:hasK_level ;
                                     owl:cardinality "1"^^xsd:nonNegativeInteger
                                   ] ,
                                   [ rdf:type owl:Restriction ;
                                     owl:onProperty ghm:hasMg_level ;
                                     owl:cardinality "1"^^xsd:nonNegativeInteger
                                   ] ,
                                   [ rdf:type owl:Restriction ;
                                     owl:onProperty ghm:hasMn_level ;
                                     owl:cardinality "1"^^xsd:nonNegativeInteger
                                   ] ,
                                   [ rdf:type owl:Restriction ;
                                     owl:onProperty ghm:hasMo_level ;
                                     owl:cardinality "1"^^xsd:nonNegativeInteger
                                   ] ,
                                   [ rdf:type owl:Restriction ;
                                     owl:onProperty ghm:hasNH4_level ;
                                     owl:cardinality "1"^^xsd:nonNegativeInteger
                                   ] ,
                                   [ rdf:type owl:Restriction ;
                                     owl:onProperty ghm:hasNO3_level ;
                                     owl:cardinality "1"^^xsd:nonNegativeInteger
                                   ] ,
                                   [ rdf:type owl:Restriction ;
                                     owl:onProperty ghm:hasNa_level ;
                                     owl:cardinality "1"^^xsd:nonNegativeInteger
                                   ] ,
                                   [ rdf:type owl:Restriction ;
                                     owl:onProperty ghm:hasP_level ;
                                     owl:cardinality "1"^^xsd:nonNegativeInteger
                                   ] ,
                                   [ rdf:type owl:Restriction ;
                                     owl:onProperty ghm:hasS_level ;
                                     owl:cardinality "1"^^xsd:nonNegativeInteger
                                   ] ,
                                   [ rdf:type owl:Restriction ;
                                     owl:onProperty ghm:hasSi_level ;
                                     owl:cardinality "1"^^xsd:nonNegativeInteger
                                   ] ,
                                   [ rdf:type owl:Restriction ;
                                     owl:onProperty ghm:hasZn_level ;
                                     owl:cardinality "1"^^xsd:nonNegativeInteger
                                   ] ,
                                   [ rdf:type owl:Restriction ;
                                     owl:onProperty ghm:haspH ;
                                     owl:cardinality "1"^^xsd:nonNegativeInteger
                                   ] ,
                                   [ rdf:type owl:Restriction ;
                                     owl:onProperty ghm:hasN_level ;
                                     owl:maxCardinality "1"^^xsd:nonNegativeInteger
                                   ] ,
                                   [ rdf:type owl:Restriction ;
                                     owl:onProperty ghm:hasN_total_level ;
                                     owl:maxCardinality "1"^^xsd:nonNegativeInteger
                                   ] ,
                                   [ rdf:type owl:Restriction ;
                                     owl:onProperty ghm:hasSugar_concentration ;
                                     owl:maxCardinality "1"^^xsd:nonNegativeInteger
                                   ] ;
                   rdfs:comment "This represents the class of nutrition levels in a sample of a fluid, e.g. water or leaf juice" ;
                   rdfs:label "Nutrition level" .


###  https://www.tno.nl/agrifood/ontology/greenhouse-model/PlantGrowth
ghm:PlantGrowth rdf:type owl:Class ;
                rdfs:subClassOf [ rdf:type owl:Restriction ;
                                  owl:onProperty ghm:hasLength ;
                                  owl:cardinality "1"^^xsd:nonNegativeInteger
                                ] ,
                                [ rdf:type owl:Restriction ;
                                  owl:onProperty ghm:hasNumberOfLeavesPerStem ;
                                  owl:maxCardinality "1"^^xsd:nonNegativeInteger
                                ] ,
                                [ rdf:type owl:Restriction ;
                                  owl:onProperty ghm:hasPlantNumber ;
                                  owl:maxCardinality "1"^^xsd:nonNegativeInteger
                                ] ,
                                [ rdf:type owl:Restriction ;
                                  owl:onProperty ghm:hasStemThickness ;
                                  owl:maxCardinality "1"^^xsd:nonNegativeInteger
                                ] ;
                rdfs:comment "This class represents growth measurements of a single plant" ;
                rdfs:label "plant growth" .


###  https://www.tno.nl/agrifood/ontology/greenhouse-model/PlantGrowthMeasurement
ghm:PlantGrowthMeasurement rdf:type owl:Class ;
                           rdfs:subClassOf owl:Thing ,
                                           [ rdf:type owl:Restriction ;
                                             owl:onProperty ghm:hasPlantGrowth ;
                                             owl:someValuesFrom ghm:PlantGrowth
                                           ] ,
                                           [ rdf:type owl:Restriction ;
                                             owl:onProperty ghm:isMeasuredInBlock ;
                                             owl:qualifiedCardinality "1"^^xsd:nonNegativeInteger ;
                                             owl:onClass ghm:Block
                                           ] ,
                                           [ rdf:type owl:Restriction ;
                                             owl:onProperty ghm:hasAverageLength ;
                                             owl:cardinality "1"^^xsd:nonNegativeInteger
                                           ] ,
                                           [ rdf:type owl:Restriction ;
                                             owl:onProperty ghm:hasAverageNumberOfLeavesPerStem ;
                                             owl:cardinality "1"^^xsd:nonNegativeInteger
                                           ] ,
                                           [ rdf:type owl:Restriction ;
                                             owl:onProperty ghm:hasAverageStemThickness ;
                                             owl:cardinality "1"^^xsd:nonNegativeInteger
                                           ] ,
                                           [ rdf:type owl:Restriction ;
                                             owl:onProperty ghm:hasDate ;
                                             owl:cardinality "1"^^xsd:nonNegativeInteger
                                           ] ,
                                           [ rdf:type owl:Restriction ;
                                             owl:onProperty ghm:hasLeafColor ;
                                             owl:cardinality "1"^^xsd:nonNegativeInteger
                                           ] ,
                                           [ rdf:type owl:Restriction ;
                                             owl:onProperty ghm:hasRootColor ;
                                             owl:cardinality "1"^^xsd:nonNegativeInteger
                                           ] ,
                                           [ rdf:type owl:Restriction ;
                                             owl:onProperty ghm:hasRootDevelopment ;
                                             owl:cardinality "1"^^xsd:nonNegativeInteger
                                           ] ,
                                           [ rdf:type owl:Restriction ;
                                             owl:onProperty ghm:hasUniformity ;
                                             owl:cardinality "1"^^xsd:nonNegativeInteger
                                           ] ;
                           rdfs:comment "This represents a measurement of the individual growth of a set of plants as well as some general parameters over the entire set, such as average length or color. " ;
                           rdfs:label "Plant growth measurement" .


###  https://www.tno.nl/agrifood/ontology/greenhouse-model/System
ghm:System rdf:type owl:Class ;
           rdfs:subClassOf owl:Thing ;
           rdfs:label "System" .


###  https://www.tno.nl/agrifood/ontology/greenhouse-model/Trait
ghm:Trait rdf:type owl:Class ;
          rdfs:subClassOf owl:Thing ;
          rdfs:comment "A trait is a characteristic of an individual plant or a group of plants that can be observed and that results from the expression of its genes and their interaction with the environment." ,
                       "Examples of a trait are: fruit shape, seed color, stem diameter, seed length, ...." ;
          rdfs:label "Trait" .


###  https://www.tno.nl/agrifood/ontology/greenhouse-model/Valve
ghm:Valve rdf:type owl:Class ;
          rdfs:subClassOf owl:Thing ;
          rdfs:label "Valve" .


###  https://www.tno.nl/agrifood/ontology/greenhouse-model/WaterAnalysis
ghm:WaterAnalysis rdf:type owl:Class ;
                  rdfs:subClassOf owl:Thing ,
                                  [ rdf:type owl:Restriction ;
                                    owl:onProperty ghm:hasNutritionLevel ;
                                    owl:qualifiedCardinality "1"^^xsd:nonNegativeInteger ;
                                    owl:onClass ghm:NutritionLevel
                                  ] ,
                                  [ rdf:type owl:Restriction ;
                                    owl:onProperty ghm:hasDate ;
                                    owl:cardinality "1"^^xsd:nonNegativeInteger
                                  ] ,
                                  [ rdf:type owl:Restriction ;
                                    owl:onProperty ghm:hasNutritionRecipe ;
                                    owl:cardinality "1"^^xsd:nonNegativeInteger
                                  ] ,
                                  [ rdf:type owl:Restriction ;
                                    owl:onProperty ghm:hasSampleName ;
                                    owl:cardinality "1"^^xsd:nonNegativeInteger
                                  ] ,
                                  [ rdf:type owl:Restriction ;
                                    owl:onProperty ghm:hasWeekDay ;
                                    owl:cardinality "1"^^xsd:nonNegativeInteger
                                  ] ,
                                  [ rdf:type owl:Restriction ;
                                    owl:onProperty ghm:hasWeekNumber ;
                                    owl:cardinality "1"^^xsd:nonNegativeInteger
                                  ] ;
                  rdfs:comment "This class represents analysis on nutritions in a sample of water that is used to irrigate plants in a greenhouse" ;
                  rdfs:label "Water analysis" .


###  https://www.tno.nl/agrifood/ontology/greenhouse-model/WaterStorageSystem
ghm:WaterStorageSystem rdf:type owl:Class ;
                       rdfs:subClassOf ghm:WaterSystem ;
                       rdfs:label "Water storage system" .


###  https://www.tno.nl/agrifood/ontology/greenhouse-model/WaterSystem
ghm:WaterSystem rdf:type owl:Class ;
                rdfs:subClassOf ghm:System ;
                rdfs:comment "This class represents the systems in the greenhouse that deal with water. This includes the infrastructure of the systems as well as the management functionality." ;
                rdfs:label "Water system" .


###  https://www.tno.nl/agrifood/ontology/greenhouse-model/Zone
ghm:Zone rdf:type owl:Class ;
         rdfs:subClassOf owl:Thing ,
                         [ rdf:type owl:Restriction ;
                           owl:onProperty ghm:contains ;
                           owl:someValuesFrom ghm:IrrigationValve
                         ] ;
         rdfs:comment "A zone is an area in which the same irrigation and fertilization strategy is applied" ;
         rdfs:label "Zone" .


#################################################################
#    Individuals
#################################################################

###  https://www.tno.nl/agrifood/ontology/greenhouse-model/snoeptomaatje
ghm:snoeptomaatje rdf:type owl:NamedIndividual ,
                           ghm:Crop ;
                  rdfs:label "snoeptomaatje" .


###  Generated by the OWL API (version 4.5.9.2019-02-01T07:24:44Z) https://github.com/owlcs/owlapi
